expose secretbox functions

code/nacl-box/Hacl.NaCl.fst
@@ -9,11 +9,92 @@ open Lib.Buffer
 open Lib.ByteBuffer
 
 module ST = FStar.HyperStack.ST
-module Spec = Spec.Box
 module LSeq = Lib.Sequence
+module SB = Spec.Box
+module SS = Spec.SecretBox
 
 
 #set-options "--max_fuel 50 --max_fuel 0 --max_ifuel 0"
+
+val crypto_secretbox_detached:
+    c:buffer uint8
+  -> tag:lbuffer uint8 16ul
+  -> m:buffer uint8
+  -> mlen:size_t{length c = v mlen /\ length m = v mlen}
+  -> n:lbuffer uint8 24ul
+  -> k:lbuffer uint8 32ul ->
+  Stack size_t
+  (requires fun h ->
+    live h c /\ live h m /\ live h k /\ live h n /\ live h tag /\
+    disjoint tag c /\ eq_or_disjoint (m <: lbuffer uint8 mlen) (c <: lbuffer uint8 mlen) /\
+    disjoint tag m /\ disjoint n m /\ disjoint n c)
+  (ensures  fun h0 r h1 -> modifies2 c tag h0 h1 /\
+    (as_seq h1 tag, as_seq #MUT #uint8 #mlen h1 c) == SS.secretbox_detached (as_seq h0 k) (as_seq h0 n) (as_seq #MUT #uint8 #mlen h0 m))
+
+let crypto_secretbox_detached c tag m mlen n k =
+  Hacl.Impl.SecretBox.secretbox_detached mlen c tag k n m;
+  0ul
+
+
+val crypto_secretbox_open_detached:
+    m:buffer uint8
+  -> c:buffer uint8
+  -> tag:lbuffer uint8 16ul
+  -> mlen:size_t{length c = v mlen /\ length m = v mlen}
+  -> n:lbuffer uint8 24ul
+  -> k:lbuffer uint8 32ul ->
+  Stack size_t
+  (requires fun h ->
+    live h c /\ live h m /\ live h k /\ live h n /\ live h tag /\
+    disjoint tag c /\ eq_or_disjoint (m <: lbuffer uint8 mlen) (c <: lbuffer uint8 mlen) /\
+    disjoint tag m /\ disjoint n m /\ disjoint n c)
+  (ensures  fun h0 r h1 -> modifies1 m h0 h1 /\
+   (let msg = SS.secretbox_open_detached (as_seq h0 k) (as_seq h0 n) (as_seq h0 tag) (as_seq #MUT #uint8 #mlen h0 c) in
+    match r with
+    | 0ul -> Some? msg /\ as_seq #MUT #uint8 #mlen h1 m == Some?.v msg
+    | _ -> None? msg))
+
+let crypto_secretbox_open_detached m c tag mlen n k =
+  Hacl.Impl.SecretBox.secretbox_open_detached mlen m k n c tag
+
+
+val crypto_secretbox_easy:
+    c:buffer uint8
+  -> m:buffer uint8
+  -> mlen:size_t{length c = v mlen + 16 /\ length m = v mlen}
+  -> n:lbuffer uint8 24ul
+  -> k:lbuffer uint8 32ul ->
+  Stack size_t
+  (requires fun h ->
+    live h c /\ live h m /\ live h k /\ live h n /\
+    disjoint m c /\ disjoint n m /\ disjoint n c)
+  (ensures  fun h0 r h1 -> modifies1 c h0 h1 /\
+    as_seq #MUT #uint8 #(mlen +! 16ul) h1 c ==
+      SS.secretbox_easy (as_seq h0 k) (as_seq h0 n) (as_seq #MUT #uint8 #mlen h0 m))
+
+let crypto_secretbox_easy c m mlen n k =
+  Hacl.Impl.SecretBox.secretbox_easy mlen c k n m;
+  0ul
+
+
+val crypto_secretbox_open_easy:
+    m:buffer uint8
+  -> c:buffer uint8
+  -> clen:size_t{length c = v clen /\ v clen = length m + 16}
+  -> n:lbuffer uint8 24ul
+  -> k:lbuffer uint8 32ul ->
+  Stack size_t
+  (requires fun h ->
+    live h c /\ live h m /\ live h k /\ live h n /\
+    disjoint m c /\ disjoint m n /\ disjoint c n)
+  (ensures fun h0 r h1 -> modifies1 m h0 h1 /\
+   (let msg = SS.secretbox_open_easy (as_seq h0 k) (as_seq h0 n) (as_seq #MUT #uint8 #clen h0 c) in
+    match r with
+    | 0ul -> Some? msg /\ as_seq #MUT #uint8 #(clen -! 16ul) h1 m == Some?.v msg
+    | _ -> None? msg))
+
+let crypto_secretbox_open_easy m c clen n k =
+  Hacl.Impl.SecretBox.secretbox_open_easy (clen -! 16ul) m k n c
 
 
 val crypto_box_beforenm:
@@ -23,8 +104,8 @@ val crypto_box_beforenm:
   Stack size_t
   (requires fun h -> live h k /\ live h pk /\ live h sk /\
     disjoint k pk /\ disjoint k sk)
-  (ensures  fun h0 r h1 -> modifies (loc k) h0 h1 /\
-   (let key = Spec.box_beforenm (as_seq h0 pk) (as_seq h0 sk) in
+  (ensures  fun h0 r h1 -> modifies1 k h0 h1 /\
+   (let key = SB.box_beforenm (as_seq h0 pk) (as_seq h0 sk) in
     match r with
     | 0ul -> Some? key /\ as_seq h1 k == Some?.v key
     | _ -> None? key))
@@ -46,7 +127,7 @@ val crypto_box_detached_afternm:
     disjoint tag c /\ eq_or_disjoint (m <: lbuffer uint8 mlen) (c <: lbuffer uint8 mlen) /\
     disjoint tag m /\ disjoint n m /\ disjoint n c)
   (ensures  fun h0 r h1 -> modifies2 c tag h0 h1 /\
-    (as_seq h1 tag, as_seq #MUT #uint8 #mlen h1 c) == Spec.box_detached_afternm (as_seq h0 k) (as_seq h0 n) (as_seq #MUT #uint8 #mlen h0 m))
+    (as_seq h1 tag, as_seq #MUT #uint8 #mlen h1 c) == SB.box_detached_afternm (as_seq h0 k) (as_seq h0 n) (as_seq #MUT #uint8 #mlen h0 m))
 
 let crypto_box_detached_afternm c tag m mlen n k =
   Hacl.Impl.Box.box_detached_afternm mlen c tag k n m
@@ -66,7 +147,7 @@ val crypto_box_detached:
     disjoint tag c /\ eq_or_disjoint (m <: lbuffer uint8 mlen) (c <: lbuffer uint8 mlen) /\
     disjoint tag m /\ disjoint n m /\ disjoint n c)
   (ensures  fun h0 r h1 -> modifies2 c tag h0 h1 /\
-   (let tag_cipher = Spec.box_detached (as_seq h0 sk) (as_seq h0 pk) (as_seq h0 n) (as_seq #MUT #uint8 #mlen h0 m) in
+   (let tag_cipher = SB.box_detached (as_seq h0 sk) (as_seq h0 pk) (as_seq h0 n) (as_seq #MUT #uint8 #mlen h0 m) in
     match r with
     | 0ul -> Some? tag_cipher /\ (let (tag_s, cipher_s) = Some?.v tag_cipher in (as_seq h1 tag, as_seq #MUT #uint8 #mlen h1 c) == (tag_s, cipher_s))
     | _ -> None? tag_cipher))
@@ -88,7 +169,7 @@ val crypto_box_open_detached_afternm:
     disjoint tag c /\ eq_or_disjoint (m <: lbuffer uint8 mlen) (c <: lbuffer uint8 mlen) /\
     disjoint tag m /\ disjoint n m /\ disjoint n c)
   (ensures  fun h0 r h1 -> modifies1 m h0 h1 /\
-   (let msg = Spec.box_open_detached_afternm (as_seq h0 k) (as_seq h0 n) (as_seq h0 tag) (as_seq #MUT #uint8 #mlen h0 c) in
+   (let msg = SB.box_open_detached_afternm (as_seq h0 k) (as_seq h0 n) (as_seq h0 tag) (as_seq #MUT #uint8 #mlen h0 c) in
     match r with
     | 0ul -> Some? msg /\ as_seq #MUT #uint8 #mlen h1 m == Some?.v msg
     | _ -> None? msg))
@@ -111,7 +192,7 @@ val crypto_box_open_detached:
     disjoint tag c /\ eq_or_disjoint (m <: lbuffer uint8 mlen) (c <: lbuffer uint8 mlen) /\
     disjoint tag m /\ disjoint n m /\ disjoint n c)
   (ensures  fun h0 r h1 -> modifies1 m h0 h1 /\
-   (let msg = Spec.box_open_detached (as_seq h0 pk) (as_seq h0 sk) (as_seq h0 n) (as_seq h0 tag) (as_seq #MUT #uint8 #mlen h0 c) in
+   (let msg = SB.box_open_detached (as_seq h0 pk) (as_seq h0 sk) (as_seq h0 n) (as_seq h0 tag) (as_seq #MUT #uint8 #mlen h0 c) in
     match r with
     | 0ul -> Some? msg /\ as_seq #MUT #uint8 #mlen h1 m == Some?.v msg
     | _ -> None? msg))
@@ -132,7 +213,7 @@ val crypto_box_easy_afternm:
     disjoint m c /\ disjoint n m /\ disjoint n c)
   (ensures  fun h0 r h1 -> modifies1 c h0 h1 /\
     as_seq #MUT #uint8 #(mlen +! 16ul) h1 c ==
-      Spec.box_easy_afternm (as_seq h0 k) (as_seq h0 n) (as_seq #MUT #uint8 #mlen h0 m))
+      SB.box_easy_afternm (as_seq h0 k) (as_seq h0 n) (as_seq #MUT #uint8 #mlen h0 m))
 
 let crypto_box_easy_afternm c m mlen n k =
   Hacl.Impl.Box.box_easy_afternm mlen c k n m
@@ -150,7 +231,7 @@ val crypto_box_easy:
     live h c /\ live h m /\ live h sk /\ live h pk /\ live h n /\
     disjoint m c /\ disjoint n m /\ disjoint n c)
   (ensures  fun h0 r h1 -> modifies1 c h0 h1 /\
-    (let cipher = Spec.box_easy (as_seq h0 sk) (as_seq h0 pk) (as_seq h0 n) (as_seq #MUT #uint8 #mlen h0 m) in
+    (let cipher = SB.box_easy (as_seq h0 sk) (as_seq h0 pk) (as_seq h0 n) (as_seq #MUT #uint8 #mlen h0 m) in
     match r with
     | 0ul -> Some? cipher /\ as_seq #MUT #uint8 #(mlen +! 16ul) h1 c == Some?.v cipher
     | _ -> None? cipher))
@@ -172,7 +253,7 @@ val crypto_box_open_easy_afternm:
     live h c /\ live h m /\ live h k /\ live h n /\
     disjoint m c /\ disjoint m n /\ disjoint c n)
   (ensures fun h0 r h1 -> modifies1 m h0 h1 /\
-   (let msg = Spec.box_open_easy_afternm (as_seq h0 k) (as_seq h0 n) (as_seq #MUT #uint8 #clen h0 c) in
+   (let msg = SB.box_open_easy_afternm (as_seq h0 k) (as_seq h0 n) (as_seq #MUT #uint8 #clen h0 c) in
     match r with
     | 0ul -> Some? msg /\ as_seq #MUT #uint8 #(clen -! 16ul) h1 m == Some?.v msg
     | _ -> None? msg))
@@ -193,7 +274,7 @@ val crypto_box_open_easy:
     live h c /\ live h m /\ live h pk /\ live h sk /\ live h n /\
     disjoint m c /\ disjoint m n /\ disjoint c n)
   (ensures fun h0 r h1 -> modifies1 m h0 h1 /\
-   (let msg = Spec.box_open_easy (as_seq h0 pk) (as_seq h0 sk) (as_seq h0 n) (as_seq #MUT #uint8 #clen h0 c) in
+   (let msg = SB.box_open_easy (as_seq h0 pk) (as_seq h0 sk) (as_seq h0 n) (as_seq #MUT #uint8 #clen h0 c) in
     match r with
     | 0ul -> Some? msg /\ as_seq #MUT #uint8 #(clen -! 16ul) h1 m == Some?.v msg
     | _ -> None? msg))
